doc/book/code/Russell.fst
@@ -30,23 +30,26 @@ let delta : set = inject delta_big
 let x_in_delta_x_not_in_delta (x:set) (mem_x_delta:mem x delta)
   : not_mem x x 
   = let (| v, r |) = mem_x_delta in // mem proofs are pairs
-    let v : (project delta).x = v in // whose first component is an element of delta's indexing set
+    let v : (project delta).x = v in // whose first component is an element of delta's comprehension domain
     let r : (x == (project delta).f v) = r in //and whose second component proves that x is equal to an element in delta
-    inj_proj delta_big; // we use the unsound axiom to conclude that `v` is actually the indexing set of delta_big
+    inj_proj delta_big; // we use the unsound axiom to conclude that `v` is actually the domain of delta_big
     let v : (s:set & not_mem s s) = v in //and now we can retype `v` this way
-    let r : (x == dfst v) = r in //and `r` this way
-    let (| _, pf |) = v in //and now the second element of v
-    let pf : not_mem x x = pf in //has the type we need
-    pf
+    let (| s, pf |) = v in //and unpack it into its components
+    let r : (x == s) = r in //and the axiom also allows us to retype `r` this way
+    let pf : not_mem x x = pf in //which lets us convert pf from `not_mem s s` to the goal
+    pf //not_mem x x
 
 let delta_not_in_delta
   : not_mem delta delta
   = fun (mem_delta_delta:mem delta delta) ->
-      x_in_delta_x_not_in_delta delta mem_delta_delta mem_delta_delta
+      x_in_delta_x_not_in_delta 
+          delta
+          mem_delta_delta
+          mem_delta_delta
 
 let x_not_mem_x_x_mem_delta (x:set) (x_not_mem_x:x `not_mem` x)
   : x `mem` delta
-  = let v : (s:set & not_mem s s) = (| x, x_not_mem_x |) in //an element of the indexing set of delta_big
+  = let v : (s:set & not_mem s s) = (| x, x_not_mem_x |) in //an element of the domain set of delta_big
     inj_proj delta_big; // the unsound axiom now lets us relate it to delta
     let s : (x == (project delta).f v) = //and prove that projecting delta's comprehension and applying to v return x`
         FStar.Squash.return_squash Refl
