doc/book/part2/part2_universes.rst
@@ -6,8 +6,8 @@ Universes
 
 As mentioned :ref:`earlier <Part1_type_of_types>`, ``Type`` is the
 type of types. So, one might ask the question, what is the type of
-``Type``? Indeed, one can write the following and it may appear at
-first that the type of ``Type`` is ``Type``.
+``Type`` itself? Indeed, one can write the following and it may appear
+at first that the type of ``Type`` is ``Type``.
 
 .. literalinclude:: ../code/Universes.fst
    :language: fstar
@@ -46,16 +46,16 @@ Other resources to learn about universes:
     <https://agda.readthedocs.io/en/latest/language/sort-system.html#sort-system>`_,
     including universe polymorphism.
 
-  * This `chapter from Adam Chlipala's *Certified Programming with
-    Dependent Types*
+  * This chapter from Adam Chlipala's `Certified Programming with
+    Dependent Types
     <http://adam.chlipala.net/cpdt/html/Cpdt.Universes.html>`_
     describes universes in Coq. While it also provides useful
-    background, F*'s universe system is more similar to Agda (and
-    Lean) than Coq.
+    background, F*'s universe system is more similar to Agda's and
+    Lean's than Coq's.
 
 
-Universes: Basics
------------------
+Basics
+------
 
 A universe annotation on a term takes the form ``u#l``, where ``l`` is
 a universe level. The universe levels are terms from the following
@@ -95,6 +95,13 @@ error:
 
    Expected expression of type "Type0"; got expression "Type0" of type "Type u#1"
 
+The restriction that prevents a ``Type`` from being an inhabitant of
+itself if sometimes called *predicativity*. The opposite,
+*impredicativity*, if not suitably restricted, usually leads to
+logical inconsistency. F* provides a limited form of impredicativity
+through the use of ``squash`` types, which we'll see towards the end
+of this chapter.
+   
 .. note::                
 
    That said, if we didn't turn on the option ``--print_universes``, the
@@ -108,17 +115,11 @@ error:
    good way to make sense of type errors where the expected type and
    the type that was computed seem identical.
 
-   The restriction that prevents a ``Type`` from being an inhabitant
-   of itself if sometimes called *predicativity*. The opposite,
-   *impredicativity*, if not suitably restricted, usually leads to
-   logical inconsistency. F* provides a limited form of
-   impredicativity through the use of ``squash`` types, which we'll
-   see towards the end of this chapter.
    
 Now, instead of defining several constants like ``ty0, ty1, ty2``
-etc., F* can be *universe polymorphic*. Below, we define ``ty_poly``
-as ``Type u#a``, for any universe variable ``a``, and so ``ty`` has
-type ``Type u#(a + 1)``. 
+etc., F* definitions can be *universe polymorphic*. Below, we define
+``ty_poly`` as ``Type u#a``, for any universe variable ``a``, and so
+``ty`` has type ``Type u#(a + 1)``.
 
 .. literalinclude:: ../code/Universes.fst
    :language: fstar
@@ -166,11 +167,11 @@ actually also polymorphic in the universe level of its type argument.
    :end-before: //SNIPPET_END: poly_id$
 
 That is, the type of the identity function ``id`` is ``id_t`` or
-``a:Type u#a -> a -> a`` or ``id_t``---meaning, for all types ``a`` in
+``a:Type u#i -> a -> a`` or ``id_t``---meaning, for all types ``a`` in
 universe ``Type u#i``, ``id a`` is function of type ``a -> a``.
 
 Now, ``id_t`` is itself a type in universe ``Type u#(i + 1)``, and
-since the ``id`` function can be applied to types in all universes, it
+since the ``id`` function can be applied to types in any universe, it
 can be applied to ``id_t`` too. So, it may look like this allows one
 to write functions that can be applied to themselves---which would be
 bad, since that would allow one to create infinite loops and break
@@ -183,7 +184,7 @@ F*'s logic.
 
 However, if we write out the universe levels explicitly, we see that
 actually we aren't really applying the ``id`` function to
-itself. Things are actually stratified, so that we applying an
+itself. Things are actually stratified, so that we are instead applying an
 instance of ``id`` at universe ``u#(i + 1)`` to the instance of ``id``
 at universes ``u#i``.
 
@@ -208,37 +209,36 @@ Universe level of an inductive type definition
 F* computes a universe level for inductive type definitions. To
 describe the rules for this in full generality, consider again the
 general form of an inductive type definition, shown first :ref:`here
-<Part2_inductives>`, but this type with the universe level of each
-type constructor made explicit, i.e., :math:`T_1` constructs a type in
-universe :math:`\mathsf{Type~u\#l_1}`
+<Part2_inductives>`, but this time with the universe level of each
+type constructor made explicit, i.e., :math:`T_i` constructs a type in
+universe :math:`\mathsf{Type~u\#l_i}`
 
 .. math::
 
-   \mathsf{type}~T_1~\overline{(x₁:p_i)} : \overline{y_1:q_1} → \mathsf{Type~u\#l_1} = \overline{| D_1 : t_1} \\
-   \mathsf{and}~T_n~\overline{(x_n:p_n)} : \overline{y_n:q_n} → \mathsf{Type~u\#l_n} =  \overline{| D_n : t_n} \\
+   \mathsf{type}~T_1~\overline{(x₁:p_i)} : \overline{y_1:q_1} → \mathsf{Type}~u\#l_1 = \overline{| D_1 : t_1} \\
+   \mathsf{and}~T_n~\overline{(x_n:p_n)} : \overline{y_n:q_n} → \mathsf{Type}~u\#l_n = \overline{| D_n : t_n} \\
 
 Recall that each type constructor :math:`T_i` has zero or more *data
 constructors* :math:`\overline{D_i:t_i}` and for each data constructor
 :math:`D_{ij}`, its type :math:`t_{ij}` must be of the form
 :math:`\overline{z_{ij}:s_{ij}} → Tᵢ~\bar{x_i}~\bar{e}`
 
-In addition to checking, as usual, that the each :math:`tᵢⱼ` is
+In addition to checking, as usual, that the each :math:`t_{ij}` is
 well-typed, F* also checks the universe levels according to the
 following rule:
 
-  * Assuming that each :math:`T_i` has universe level :math:`l_i`
-
-  * For every data constructor :math:`D_{ij}`, and for each of its
-    arguments :math:`z_{ijk} : s_{ijk}`, check :math:`s_{ijk} : \mathsf{Type~u\#l_{ijk}}` and :math:`l_{ijk} ≤ l_i`.
+  * Assuming that each :math:`T_i` has universe level :math:`l_i`, for
+    every data constructor :math:`D_{ij}`, and for each of its
+    arguments :math:`z_{ijk} : s_{ijk}`, check :math:`s_{ijk} :
+    \mathsf{Type}~u\#l_{ijk}` and :math:`l_{ijk} ≤ l_i`.
 
 In other words, the universe level of each type constructor must not
-be less than less than the universe of any of the fields of data
-constructors.
+be less than the universe of any of the fields of data constructors.
 
 In practice, F* infers the universe levels :math:`l_1, …, l_n`, by
 collecting level-inequality constraints and solving them using the
 ``max`` operator on universe levels, i.e., :math:`l_i` is set to
-:math:`max_{jk} l_{ijk}`, the maximum of the universe levels of all
+:math:`max_{jk}~l_{ijk}`, the maximum of the universe levels of all
 the fields of the constructors :math:`\overline{D_i : t_i}`. Let's
 look at some examples.
 
@@ -265,7 +265,7 @@ F* infers the minimum satisfiable universe level assignment, by
 default. But, there are many solutions to the inequalities, and if
 needed, one can use annotations to pick another solution. For example,
 one could write this, though it rarely makes sense to pick a universe
-for a type higher that necessary (see :ref:`this section <Part2_Universes_raising>` for an exception).
+for a type higher than necessary (see :ref:`this section <Part2_Universes_raising>` for an exception).
 
 .. literalinclude:: ../code/Universes.fst
    :language: fstar
@@ -305,15 +305,15 @@ with its type.
    :start-after: //SNIPPET_START: top$
    :end-before: //SNIPPET_END: top$
 
-* The ``a`` field of ``Top`` in ``u#(a + 1)`` while the ``v`` field
+* The ``a`` field of ``Top`` is in ``u#(a + 1)`` while the ``v`` field
   is in ``u#a``. So, ``top`` itself is in ``u#(max (a + 1) a)``,
   which simplifies to ``u#(a + 1)``.
 
 One intuition for why this is so is that from a value of type ``t :
 top`` one can write a function that computes a value of type ``Type
-u#a``, i.e., ``Top?.a t``. So, if, for instance we have ``top: Type
-u#a`` and ``t:top``, then ``Top?.a : top -> Type u#a``, which would
-break the stratification of universes. From a value ``top`` in
+u#a``, i.e., ``Top?.a t``. So, if instead we have ``top: Type u#a``
+and ``t:top``, then ``Top?.a : top -> Type u#a``, which would break
+the stratification of universes, since from a value ``top`` in
 universe ``u#a``, we would be able to project out a value in
 ``Type u#(a + 1)``, which leads to a paradox, as we'll see next.
 
@@ -324,7 +324,7 @@ constructed.
 Russell's Paradox
 -----------------
 
-Type theory has its roots in Bertrand Russell's work `The Principles
+Type theory has its roots in Bertrand Russell's `The Principles
 of Mathematics
 <https://en.wikipedia.org/wiki/The_Principles_of_Mathematics>`_, which
 explores the logical foundations of mathematics and set theory. In
@@ -351,7 +351,7 @@ the stratification of universes in F*, then one can code up Russell's
 :math:`\Delta` set and prove ``False``. This construction is derived
 from `Thorsten Altenkirch's Agda code
 <http://www.cs.nott.ac.uk/~psztxa/g53cfr/l20.html/l20.html>`_. Liam
-O'Connor also provides some useful context and comparison `here
+O'Connor also provides `some useful context and comparison
 <http://liamoc.net/posts/2015-09-10-girards-paradox.html>`_. Whereas
 the Agda code uses a special compiler pragma to enable unsound
 impredicativity, in F* we show how a user-introduced axiom can
@@ -361,7 +361,7 @@ simulate impredicativity and enable the same paradox.
 Breaking the Universe System
 .............................
 
-Consider the following interface that intentionally breaks the
+Consider the following axioms that intentionally break the
 stratification of F*'s universe system. We'll need the following
 ingredients:
 
@@ -396,23 +396,23 @@ ingredients:
 Encoding Russell's Paradox
 ...........................
 
-To show the paradox, we'll define a notion of ``set`` that can be
-defined by a form of set comprehensions ``f: x -> set``, where
-``x:Type u#0`` is an index to the comprehension, supposedly bounding
-the cardinality of the set.  We'll subvert the universe system by
-treating ``set`` as living in universe ``u#0``, even though they
-contain a term ``x:Type u#0`` that has universe level ``u#1``
+To show the paradox, we'll define a notion of ``set`` in terms of a
+form of set comprehensions ``f: x -> set``, where ``x:Type u#0`` is
+the domain of the comprehension, supposedly bounding the cardinality
+of the set.  We'll subvert the universe system by treating ``set`` as
+living in universe ``u#0``, even though its constructor ``Set`` has a
+field ``x:Type u#0`` that has universe level ``u#1``
 
 .. literalinclude:: ../code/Russell.fst
    :language: fstar
    :start-after: //SNIPPET_START: set$
    :end-before: //SNIPPET_END: set$
 
-This construction allows us to define many useful sets.
-
-For example, the empty set ``zero`` as no elements; or the singleton
-set ``one`` whose only element is the empty set; or the set ``two``
-that contains the empty set ``zero`` and the singleton set ``one``.
+This construction allows us to define many useful sets. For example,
+the empty set ``zero`` uses the empty type ``False`` as the domain of
+its comprehension and so has no elements; or the singleton set ``one``
+whose only element is the empty set; or the set ``two`` that contains
+the empty set ``zero`` and the singleton set ``one``.
                 
 .. literalinclude:: ../code/Russell.fst
    :language: fstar
@@ -420,12 +420,13 @@ that contains the empty set ``zero`` and the singleton set ``one``.
    :end-before: //SNIPPET_END: zero,one,two$
 
 One can also define set membership: A set ``a`` is a member of a set
-``b``, if one can exhibit an element ``v`` of the indexing type of
+``b``, if one can exhibit an element ``v`` of the domain type of
 ``b`` (i.e., ``(project b).x``), such that ``b``'s comprehension
-``(project b).f`` applied to ``v`` is ``a``. For example, on can prove
-``mem zero two`` by picking ``true`` for ``v`` and ``mem one two`` by
-picking ``false`` for ``v``. Non-membership is just the negation of
-membership.
+``(project b).f`` applied to ``v`` is ``a``.
+
+For example, one can prove ``mem zero two`` by picking ``true`` for
+``v`` and ``mem one two`` by picking ``false`` for
+``v``. Non-membership is just the negation of membership.
 
 .. literalinclude:: ../code/Russell.fst
    :language: fstar
@@ -435,9 +436,9 @@ membership.
 Now, we are ready to define Russell's paradoxical set
 :math:`\Delta`. First, we define ``delta_big`` in a larger universe
 and then use ``inject`` to turn it into a ``set : Type u#0``. The
-encoding of ``delta_big`` is fairly direct: Its indexing type are sets
-``s`` paired with proofs that ``s`` does not contain itself; and its
-comprehension function just returns ``s`` itself.
+encoding of ``delta_big`` is fairly direct: Its domain type is the
+type of sets ``s`` paired with a proof that ``s`` does not contain
+itself; and its comprehension function just returns ``s`` itself.
       
 .. literalinclude:: ../code/Russell.fst
    :language: fstar
@@ -453,16 +454,306 @@ system, and derive ``False``.
    :start-after: //SNIPPET_START: proof$
    :end-before: //SNIPPET_END: proof$
 
-Impredicativity, refinement types, and FStar.Squash
----------------------------------------------------
+The proofs are more detailed than they need to be, and if you're
+curious, maybe you can follow along by reading the comments.
+
+The upshot, however, is that without the stratification of universes,
+F* would be unsound.
+
+
+Refinement types, FStar.Squash, ``prop``, and Impredicativity
+-------------------------------------------------------------
+
+We've seen how universes levels are computed for arrow types and
+inductive type definitions. The other way in which types can be formed
+in F* is with refinement types: ``x:t{ϕ}``. As we've seen previously,
+a value ``v`` of type ``x:t{ϕ}`` is just a ``v:t`` where ``ϕ[v/x]`` is
+derivable in the current scope in F*'s SMT-assisted classical
+logic—there is no way to extract a proof of ``ϕ`` from a proof of
+``x:t{ϕ}``, i.e., refinement types are F*'s mechanism for proof
+irrelevance.
+
+**Universe of a refinement type**: The universe of a refinement type ``x:t{ϕ}`` is the universe of ``t``.
+
+Since the universe of a refinement type does not depend on ``ϕ``, it
+enables a limited form of impredicativity, and we can define the
+following type (summarized here from the F* standard library
+``FStar.Squash``):
+
+.. code-block:: fstar
+
+   let squash (p:Type u#p) : Type u#0 = _:unit { p }
+   let return_squash (p:Type u#p) (x:p) : squash p = ()
+
+This is a lot like the ``lower`` and ``inject`` assumptions that we
+saw in the previous section, but, importantly, there is no ``project``
+operation to invert an ``inject``. In fact, ``FStar.Squash`` proves
+that ``squash p`` is proof irrelevant, meaning that all proofs of
+``squash p`` are equal.
+
+.. code-block:: fstar
+
+   val proof_irrelevance (p: Type u#p) (x y: squash p) : squash (x == y)
+
+``FStar.Squash`` does provide a limited way to manipulate a proof of
+``p`` given a ``squash p``, using the combinator ``bind_squash`` shown
+below, which states that if ``f`` can build a proof ``squash b`` from any
+proof of ``a``, then it can do so from the one and only proof of ``a``
+that is witnessed by ``x:squash a``. 
+
+.. code-block:: fstar
+
+   val bind_squash (#a: Type u#a) (#b: Type u#b) (x: squash a) (f: (a -> squash b)) : squash b
+   
+It is important that ``bind_squash`` return a ``squash b``,
+maintaining the proof-irrelevance of the ``squash`` type. Otherwise,
+if one could extract a proof of ``a`` from ``squash a``, we would be
+perilously close to the unsound ``project`` axiom which enables
+paradoxes.
+
+This restriction is similar to Coq's restriction on its ``Prop`` type,
+forbidding functions match on ``Prop`` to return results outside
+``Prop``.
+
+The F* type ``prop`` (which we saw first :ref:`here <Part1_prop>`) is
+defined primitively as type of all squashed types, i.e., the only
+types in ``prop`` are types of the form ``squash p``; or,
+equivalently, every type ``t : prop``, is a subtype of ``unit``. Being
+the type of a class of types, ``prop`` in F* lives in ``u#1``
+
+.. literalinclude:: ../code/Universes.fst
+   :language: fstar
+   :start-after: //SNIPPET_START: prop$
+   :end-before: //SNIPPET_END: prop$
+
+However, ``prop`` still offers a form of impredicativity, e.g., you
+can quantify over all ``prop`` while remaining in ``prop``.
+
+.. literalinclude:: ../code/Universes.fst
+   :language: fstar
+   :start-after: //SNIPPET_START: prop impredicative$
+   :end-before: //SNIPPET_END: prop impredicative$
+
+* The first line above shows that, as usual, an arrow type is in a
+  universe that is the maximum of the universes of its argument and
+  result types. In this case, since it has an argument ``prop : Type
+  u#1`` the arrow itself is in ``u#1``.
+
+* The second line shows that by squashing the arrow type, we can bring
+  it back to ``u#0``
+
+* The third line shows the more customary way of doing this in F*,
+  where ``forall (a:prop). a`` is just syntactic sugar for ``squash
+  (a:prop -> a)``. Since this is a ``squash`` type, not only does it
+  live in ``Type u#0``, it is itself a ``prop``.
+
+* The fourth line shows that the same is true for ``exists``.
 
 .. _Part2_Universes_raising:
 
-Raising universes, or the lack of cumulativity
+Raising universes and the lack of cumulativity
 ----------------------------------------------
 
+In some type theories, notably in Coq, the universe system is
+*cumulative*, meaning that ``Type u#i : Type u#(max (i + i) j)``;
+or, that ``Type u#i`` inhabits all universes greater than
+``i``. In contrast, in F*, as in Agda and Lean, ``Type u#i : Type
+u#(i + 1)``, i.e., a type resides only in the universe immediately
+above it.
 
-Universe Inference: Annotations and conventions
------------------------------------------------
+Cumulativity is a form of subtyping on universe levels, and it can be
+quite useful, enabling definitions at higher universes to be re-used
+for all lower universes. However, systems that mix universe
+polymorphism with cumulativity are quite tricky, and indeed, it was
+only recently that Coq offered both universe polymorphism and
+cumulativity.
 
+Lacking cumulativity, F* provides a library ``FStar.Universe`` that
+enables lifting a term from one universe to a higher one. We summarize
+it here:
 
+.. code-block:: fstar
+
+   val raise_t ([@@@ strictly_positive] t : Type u#a) : Type u#(max a b)
+
+   val raise_val (#a:Type u#a) (x:a) : raise_t u#a u#b a
+
+   val downgrade_val (#a:Type u#a) (x:raise_t u#a u#b a) : a
+
+   val downgrade_val_raise_val (#a: Type u#a) (x: a)
+     : Lemma (downgrade_val u#a u#b (raise_val x) == x)
+
+   val raise_val_downgrade_val (#a: Type u#a) (x: raise_t u#a u#b a)
+     : Lemma (raise_val (downgrade_val x) == x)
+
+The type ``raise_t t`` is strictly positive in ``t`` and raises ``t``
+from ``u#a`` to ``u#(max a b)``. ``raise_val`` and
+``downgrade_val`` are mutually inverse functions between ``t`` and
+``raise_t t``.
+
+This signature is similar in structure to the unsound signature for
+``lower, inject, project`` that we use to exhibit Russell's
+paradox. However, crucially, the universe levels in ``raise_t`` ensure
+that the universe levels *increase*, preventing any violation of
+universe stratification.
+
+In fact, this signature is readily implemented in F*, as shown below,
+where the universe annotation on ``raise_t`` explicitly defines the
+type in a higher universe ``u#(max a b)`` rather than in its minimum
+universe ``u#a``.
+
+.. code-block:: fstar
+
+  noeq
+  type raise_t (a : Type u#a) : Type u#(max a b) =
+    | Ret : a -> raise_t a
+
+  let raise_val #a x = Ret x
+  let downgrade_val #a x = match x with Ret x0 -> x0
+  let downgrade_val_raise_val #a x = ()
+  let raise_val_downgrade_val #a x = ()
+
+.. _Part2_tips_for_universes:  
+
+Tips for working with universes
+-------------------------------
+
+Whenever you write ``Type`` in F*, you are implicitly writing ``Type
+u#?x``, where ``?x`` is a universe *metavariable* left for F* to infer. When
+left implicit, this means that F* may sometimes infer universes for
+your definition that are not what you expect---they may be too general
+or not general enough. We conclude this section with a few tips to
+detect and fix such problems.
+
+* If you see puzzling error messages, enable the following pragma:
+
+  .. code-block:: fstar
+
+     #push-options "--print_implicits --print_universes"
+
+  This will cause F* to print larger terms in error messages, which
+  you usually do not want, except when you are confronted with error
+  messages of the form "expected type t; got type t".
+
+* Aside from the built-in constants ``Type u#a``, the ``->`` type
+  constructor, and the refinement type former, the only universe
+  polymorphic F* terms are top-level definitions. That is, while you
+  can define ``i`` at the top-level and use it polymorphically:
+
+  .. literalinclude:: ../code/Universes.fst
+     :language: fstar
+     :start-after: //SNIPPET_START: id_top_level$
+     :end-before: //SNIPPET_END: id_top_level$
+
+  You cannot do the same in a non-top-level scope:
+  
+  .. literalinclude:: ../code/Universes.fst
+     :language: fstar
+     :start-after: //SNIPPET_START: no_local_poly$
+     :end-before: //SNIPPET_END: no_local_poly$
+
+  Of course, non-universe-polymorphic definitions work at all scopes,
+  e.g., here, the ``i`` is polymorphic in all types at universe
+  ``u#0``.
+
+  .. literalinclude:: ../code/Universes.fst
+     :language: fstar
+     :start-after: //SNIPPET_START: type_poly$
+     :end-before: //SNIPPET_END: type_poly$
+
+* If you write a ``val f : t`` declaration for ``f``, F* will compute
+  the most general universe for the type ``t`` independently of the
+  ``let f = e`` or ``type f =`` definition.
+
+  A simple example of this behavior is the following. Say, you declare
+  ``tup2`` as below.
+
+  .. literalinclude:: ../code/Universes.fst
+     :language: fstar
+     :start-after: //SNIPPET_START: val tup2$
+     :end-before: //SNIPPET_END: val tup2$
+
+  Seeing this declaration F* infers ``val tup2 (a:Type u#a) (b:Type u#b)
+  : Type u#c``, computing the most general type for ``tup2``.
+
+  If you now try to define ``tup2``, 
+
+  .. literalinclude:: ../code/Universes.fst
+     :language: fstar
+     :start-after: //SNIPPET_START: let tup2$
+     :end-before: //SNIPPET_END: let tup2$
+
+  F* complains with the following error (with ``--print_universes`` on):
+
+  .. code-block::
+
+     Type u#(max uu___43588 uu___43589) is not a subtype of the expected type Type u#uu___43590
+     
+  Meaning that the inferred type for the definition of ``tup2 a b`` is
+  ``Type u#(max a b)``, which is of course not the same a ``Type
+  u#c``, and, sadly, the auto-generated fresh names in the error
+  message don't make your life any easier.
+
+  The reason for this is that one can write a ``val f : t`` in a
+  context where a definition for ``f`` may never appear, in which case
+  F* has to compute some universes for ``t``---it chooses the most
+  general universe, though if you do try to implement ``f`` you may
+  find that the most general universe is too general.
+
+  A good rule of thumb is the following:
+
+  - Do not write a ``val`` declaration for a term, unless you are
+    writing an :ref:`interface <Part3_interfaces>`. Instead, directly
+    write a ``let`` or ``type`` definition and annotate it with the
+    type you expect it to have---this will lead to fewer
+    surprises. For example, instead of separating the ``val tup2``
+    from ``let tup2`` just write them together, as shown below, and F*
+    infers the correct universes.
+
+    .. literalinclude:: ../code/Universes.fst
+       :language: fstar
+       :start-after: //SNIPPET_START: tuple2$
+       :end-before: //SNIPPET_END: tuple2$
+
+  - If you must write a ``val f : t``, because, say, the type ``t`` is
+    huge, or because you are writing an inferface, it's a good idea to
+    be explicit about universes, so that when defining ``f``, you know
+    exactly how general you have to be in terms of universes; and,
+    conversely, users of ``f`` know exactly how much universe
+    polymorphism they are getting. For example:
+
+    .. literalinclude:: ../code/Universes.fst
+       :language: fstar
+       :start-after: //SNIPPET_START: tup2_again$
+       :end-before: //SNIPPET_END: tup2_again$
+
+* When defining an inductive type, prefer using parameters over
+  indexes, since usually type parameters lead to types in lower
+  universes. For example, one might think to define lists this way:
+
+  .. literalinclude:: ../code/Universes.fst
+     :language: fstar
+     :start-after: //SNIPPET_START: list_alt$
+     :end-before: //SNIPPET_END: list_alt$
+
+  Although semantically equivalent to the standard list        
+
+  .. literalinclude:: ../code/Universes.fst
+     :language: fstar
+     :start-after: //SNIPPET_START: list$
+     :end-before: //SNIPPET_END: list$
+
+  ``list_alt`` produces a type in ``u#(a + 1)``, since both ``NilAlt``
+  and ``ConsAlt`` have fields of type ``a:Type u#a``. So, unless the
+  index of your type varies among the constructors, use a parameter
+  intead of an index.
+  
+  That said, recall that it's the fields of the constructors of the
+  inductive type that count. You can index your type by a type in any
+  universe and it doesn't influence the result type. Here's an
+  artificial example.
+
+  .. literalinclude:: ../code/Universes.fst
+     :language: fstar
+     :start-after: //SNIPPET_START: crazy_index$
+     :end-before: //SNIPPET_END: crazy_index$
