doc/book/part3/part3_interfaces.rst
@@ -233,6 +233,10 @@ is the following:
     contains ``val f : tf`` followed by ``val g : tg``, then the
     implementation of ``f`` must precede the implementation of ``g``.
 
+Also, remember that if you are writing ``val`` declaration in an
+interface, it is a good idea to be explicit about universe levels. See
+:ref:`here for more discussion <Part2_tips_for_universes>`.
+
 Other issues with interleaving that may help in debugging compiler
 errors with interfaces:
 
